src/lib/sparse/Kuiper.Sparse.SPMM.Compute.fsti
@@ -8,11 +8,10 @@ open Kuiper.Seq.Common { (@+) }
 open Kuiper.Spec.GEMM
 open Kuiper.Sparse.DotProduct
 open Kuiper.Sparse.Common
-open Kuiper.Sparse.SPMM.Defs { ematrix_tile_prop }
+open Kuiper.Sparse.SPMM.Defs { chest2_tile_prop }
 open Kuiper.Array.Vectorized
-open Kuiper.Tensor { ctlayout }
-module A = Kuiper.Array1
-module M = Kuiper.Array2
+open Kuiper.Tensor
+open Kuiper.Seq.Common { op_At_Bang }
 
 
 val tile_vmprod_prop
@@ -22,7 +21,7 @@ val tile_vmprod_prop
   (elems : erased (lseq et m1))
   (row_ind : erased (lseq nat m1))
   (#m2 #n2 : nat {  chunk et /? n2 })
-  (em2 : ematrix et m2 n2)
+  (em2 : chest2 et m2 n2)
   (j : nat { chunk et /? j })
   (step : nat)
   (#_ : squash (in_bounds 0 m2 row_ind))
@@ -36,7 +35,7 @@ val tile_vmprod_prop_lemma0
   (elems : erased (lseq et m1))
   (row_ind : erased (lseq nat m1))
   (#m2 #n2 : nat {  chunk et /? n2 })
-  (em2 : ematrix et m2 n2)
+  (em2 : chest2 et m2 n2)
   (j : nat { chunk et /? j })
   (step : nat)
   (#_ : squash (in_bounds 0 m2 row_ind))
@@ -47,14 +46,14 @@ val tile_vmprod_prop_lemma0
 val tile_mask_lemma
   (#et : Type0) {| scalar et, sized et, has_vec_cpy et |}
   (#rows #shared #cols : nat { chunk et /? cols })
-  (em1 : ematrix et rows shared)
+  (em1 : chest2 et rows shared)
   (i : natlt rows)
   (#nnz : nat)
   (mask_len : natle nnz)
   (elems : erased (lseq et (nnz - mask_len)))
   (row_ind : erased (lseq nat nnz))
   (#_ : squash (in_bounds 0 shared row_ind /\ sorted row_ind))
-  (em2 : ematrix et shared cols)
+  (em2 : chest2 et shared cols)
   (j : nat { chunk et /? j })
   (step : nat)
   (#tlen : nat { chunk et /? tlen })
@@ -78,9 +77,9 @@ val tile_mask_lemma
 let tile_result_cell_prop
   (#et : Type0) {| scalar et, sized et, has_vec_cpy et |}
   (#rows #shared #cols : nat)
-  (em1 : ematrix et rows shared)
+  (em1 : chest2 et rows shared)
   (i : natlt rows)
-  (em2 : ematrix et shared cols)
+  (em2 : chest2 et shared cols)
   (j : nat)
   (step : nat)
   (#tlen : nat)
@@ -95,9 +94,9 @@ let tile_result_cell_prop
 let tile_result_prop
   (#et : Type0) {| scalar et, sized et, has_vec_cpy et |}
   (#rows #shared #cols : nat)
-  (em1 : ematrix et rows shared)
+  (em1 : chest2 et rows shared)
   (i : natlt rows)
-  (em2 : ematrix et shared cols)
+  (em2 : chest2 et shared cols)
   (j : nat)
   (step : nat)
   (#tlen : nat)
@@ -110,13 +109,13 @@ let tile_result_prop
 val tile_result_lemma
   (#et : Type0) {| scalar et, sized et, has_vec_cpy et |}
   (#rows #shared #cols : nat { chunk et /? cols })
-  (em1 : ematrix et rows shared)
+  (em1 : chest2 et rows shared)
   (i : natlt rows)
   (#nnz : nat)
   (elems : erased (lseq et nnz))
   (row_ind : erased (lseq nat nnz))
   (#_ : squash (in_bounds 0 shared row_ind /\ sorted row_ind))
-  (em2 : ematrix et shared cols)
+  (em2 : chest2 et shared cols)
   (j : nat { chunk et /? j })
   (step : nat)
   (#tlen : nat { chunk et /? tlen })
@@ -137,31 +136,31 @@ inline_for_extraction noextract
 fn tile_vmprod
   (#et : Type0) {| scalar et, sized et, hvc : has_vec_cpy et |}
   (#m1 #n1 : sz { chunk et /? n1 })
-  (#ly : A.layout n1) {| ctlayout ly |}
-  (y : A.array1 et ly)
-  (#vy : erased (lseq et n1))
+  (#ly : layout1 n1) {| ctlayout ly |}
+  (y : array1 et ly)
+  (#vy : chest1 et n1)
   (vy0 : erased (lseq et n1))
-  (#lx : A.layout m1) {| ctlayout lx |}
-  (x : A.array1 et lx)
+  (#lx : layout1 m1) {| ctlayout lx |}
+  (x : array1 et lx)
   (#fx : perm)
   (#nnz : erased nat)
   (elems : erased (lseq et nnz))
   (row_ind : erased (lseq nat nnz))
   (to : erased nat { to + m1 <= nnz })
-  (#ltm : M.layout m1 n1) {| ctlayout ltm |}
-  (tm : M.array2 et ltm)
-  (#tem : ematrix et m1 n1)
+  (#ltm : layout2 m1 n1) {| ctlayout ltm |}
+  (tm : array2 et ltm)
+  (#tem : chest2 et m1 n1)
   (#ftm : perm)
   (#m2 #n2 : nat {  chunk et /? n2 })
-  (gem : ematrix et m2 n2)
+  (gem : chest2 et m2 n2)
   (j : sz { chunk et /? j })
   (step : sz)
   (#_ : squash (in_bounds 0 m2 row_ind /\ sorted row_ind))
   norewrite
   preserves gpu
-  preserves x  |-> Frac fx (Seq.slice elems to (to + m1) <: lseq et m1)
+  preserves x  |-> Frac fx (seq_to_chest1 (Seq.slice elems to (to + m1) <: lseq et m1))
   preserves tm |-> Frac ftm tem
-  requires  pure (ematrix_tile_prop #_ #_ #hvc gem (Seq.slice row_ind to (to + m1)) j step tem)
+  requires  pure (chest2_tile_prop #_ #_ #hvc gem (Seq.slice row_ind to (to + m1)) j step tem)
   requires  y  |-> vy
   requires
     pure (
@@ -170,9 +169,9 @@ fn tile_vmprod
         (Seq.slice elems 0 to <: lseq et to) (Seq.slice row_ind 0 to)
         gem
         j step
-        vy
+        (chest1_to_seq vy)
     )
-  ensures exists* (vy' : lseq et n1).
+  ensures exists* (vy' : chest1 et n1).
     y |-> vy' **
     pure (
       tile_vmprod_prop
@@ -180,7 +179,7 @@ fn tile_vmprod
         (Seq.slice elems 0 (to + m1) <: lseq et (to + m1)) (Seq.slice row_ind 0 (to + m1))
         gem
         j step
-        vy'
+        (chest1_to_seq vy')
     )
 
 open Kuiper.Array2.Strided { strided_row_major, aligned_strided_row_major }
@@ -189,33 +188,33 @@ inline_for_extraction noextract
 fn tile_load_vmprod
   (#et : Type0) {| scalar et, sized et, has_vec_cpy et |}
   (#m1 #n1 : sz { chunk et /? n1 })
-  (#ly : A.layout n1) {| ctlayout ly |}
+  (#ly : layout1 n1) {| ctlayout ly |}
   // en realidad y es un larray... por el momento no podemos unificar
-  (y : A.array1 et ly)
-  (#vy : erased (lseq et n1))
+  (y : array1 et ly)
+  (#vy : chest1 et n1)
   (vy0 : erased (lseq et n1))
-  (#lx  : A.layout m1) {| ctlayout lx |}
-  (elems : A.array1 et lx)
-  (row_ind : A.array1 sz lx)
+  (#lx  : layout1 m1) {| ctlayout lx |}
+  (elems : array1 et lx)
+  (row_ind : array1 sz lx)
   (#fx : perm)
   (#nnz : erased nat)
   (#velems : lseq et nnz)
   (#vrow_ind : lseq sz nnz)
   (#m2 #n2 : szp { chunk et /? n2 })
-  (#lm : M.layout m2 n2) {| ctlayout lm, srm : strided_row_major lm |}
-  (m : M.array2 et lm)
+  (#lm : layout2 m2 n2) {| ctlayout lm, srm : strided_row_major lm |}
+  (m : array2 et lm)
   (#fm : perm)
-  (#em : ematrix et m2 n2)
+  (#em : chest2 et m2 n2)
   (j : sz { chunk et /? j })
   (step : sz)
   (#_ : squash (in_bounds 0 m2 (cast_pos vrow_ind)))
   (from to : erased nat { from + m1 <= nnz })
   (cant : szlt m1 { v cant == to - from })
   preserves gpu
-  preserves elems   |-> Frac fx (Seq.slice velems from (from + m1) <: lseq et m1)
-  preserves row_ind |-> Frac fx (Seq.slice vrow_ind from (from + m1) <: lseq sz m1)
+  preserves elems   |-> Frac fx (seq_to_chest1 (Seq.slice velems from (from + m1) <: lseq et m1))
+  preserves row_ind |-> Frac fx (seq_to_chest1 (Seq.slice vrow_ind from (from + m1) <: lseq sz m1))
   preserves m |-> Frac fm em
-  requires  pure (aligned 16 (M.core m) /\ aligned_strided_row_major (chunk et) srm)
+  requires  pure (aligned 16 (core m) /\ aligned_strided_row_major (chunk et) srm)
   requires  pure (fits (j + n1 * step))
   requires  y |-> vy
   requires
@@ -226,14 +225,14 @@ fn tile_load_vmprod
         (Seq.slice (cast_pos vrow_ind) 0 from)
         em
         j step
-        vy
+        (chest1_to_seq vy)
     )
-  ensures exists* vy'.
+  ensures exists* (vy' : chest1 et n1).
     y |-> vy' **
     pure (
       tile_vmprod_prop
         vy0
         (Seq.slice velems 0 to <: lseq et to)
         (Seq.slice (cast_pos vrow_ind) 0 to <: lseq nat to)
-        em j step vy'
+        em j step (chest1_to_seq vy')
     )
