src/lib/sparse/Kuiper.Sparse.SPMM.fsti
@@ -23,25 +23,25 @@ fn spmm
     (k * chunk et) /? blockItemsX
   }))
   (blockChunks : sz{SZ.v blockChunks == blockItemsX / blockWidth}) // Ver nota abajo
-  (#lB : Array2.layout shared cols) {| ctlayout lB, srmB : strided_row_major lB |}
-  (#lC : Array2.layout rows cols)   {| ctlayout lC, srmC : strided_row_major lC |}
+  (#lB : layout2 shared cols) {| ctlayout lB, srmB : strided_row_major lB |}
+  (#lC : layout2 rows cols)   {| ctlayout lC, srmC : strided_row_major lC |}
   (gA : smatrix et (SZ.v rows) (SZ.v shared){is_global_smatrix gA})
   (#_ : squash (aligned 16 gA.elems /\ aligned 16 gA.col_ind))
   (#fA : perm)
   (row_indices : larray sz rows)
   (fri : perm)
-  (gB : Array2.t et lB{Array2.is_global gB})
-  (#_ : squash (aligned 16 (Array2.core gB)))
+  (gB : array2 et lB{is_global gB})
+  (#_ : squash (aligned 16 (core gB)))
   (#_ : squash (aligned_strided_row_major (chunk et) srmB))
   (#fB : perm)
-  (gC : Array2.t et lC{Array2.is_global gC})
-  (#_ : squash (aligned 16 (Array2.core gC)))
+  (gC : array2 et lC{is_global gC})
+  (#_ : squash (aligned 16 (core gC)))
   (#_ : squash (aligned_strided_row_major (chunk et) srmC))
   // matriz sparse gA
   (elems : erased (lseq et gA.nnz))
   (col_ind : erased (lseq sz gA.nnz))
   (row_off : erased (lseq sz (rows + 1)))
-  (#eA : ematrix et rows shared)
+  (#eA : chest2 et rows shared)
   // permutacion de filas
   (row_perm : permutation (natlt rows))
   // matrices densas
